fix(libs/core,libs/rust_primitives): misc

libs/fstar/core/Core.Iter.fsti
@@ -38,14 +38,14 @@ instance iterator_enumerate it {| i: iterator it |}: iterator (Core.Iter.Adapter
 (** Slices are not iterable as such in Rust. We ignore this indirection here. *)
 open Core.Ops.Range
 
-val iterator_slice_next t: t_next (slice t) t
+val iterator_slice_next t: t_next (t_Slice t) t
 unfold
-let iterator_slice_contains (t: eqtype): t_contains (slice t) t
+let iterator_slice_contains (t: eqtype): t_contains (t_Slice t) t
   = fun s x -> Rust_primitives.Arrays.contains s x
-val iterator_slice_fold (t: eqtype): t_fold (slice t) t (iterator_slice_contains t)
-val iterator_slice_enumerate (t: eqtype): t_enumerate (slice t)
+val iterator_slice_fold (t: eqtype): t_fold (t_Slice t) t (iterator_slice_contains t)
+val iterator_slice_enumerate (t: eqtype): t_enumerate (t_Slice t)
 
-instance iterator_slice (t: eqtype): iterator (slice t) = {
+instance iterator_slice (t: eqtype): iterator (t_Slice t) = {
   f_Item = t;
   f_next = iterator_slice_next t;
   // size_hint = (fun s -> Some (Rust_primitives.Arrays.length s));
@@ -56,17 +56,17 @@ instance iterator_slice (t: eqtype): iterator (slice t) = {
 
 (**** Array *)
 (** Arrays are not iterable as such in Rust. We ignore this indirection here. *)
-val iterator_array_next t len: t_next (array t len) t
+val iterator_array_next t len: t_next (t_Array t len) t
 unfold
-let iterator_array_contains (t: eqtype) len: t_contains (array t len) t
+let iterator_array_contains (t: eqtype) len: t_contains (t_Array t len) t
   = fun s x -> Rust_primitives.Arrays.contains s x
-val iterator_array_fold (t: eqtype) len: t_fold (array t len) t (iterator_array_contains t len)
-val iterator_array_enumerate (t: eqtype) len: t_enumerate (array t len)
+val iterator_array_fold (t: eqtype) len: t_fold (t_Array t len) t (iterator_array_contains t len)
+val iterator_array_enumerate (t: eqtype) len: t_enumerate (t_Array t len)
 
-instance iterator_array (t: eqtype) len: iterator (array t len) = {
+instance iterator_array (t: eqtype) len: iterator (t_Array t len) = {
   f_Item = t;
   f_next = iterator_array_next t len;
-  // size_hint = (fun (_s: array t len) -> Some len);
+  // size_hint = (fun (_s: t_Array t len) -> Some len);
   f_contains  = iterator_array_contains  t len;
   f_fold      = iterator_array_fold      t len;
   f_enumerate = iterator_array_enumerate t len;
