libs/fstar/core/Core.Slice.Iter.fst
@@ -2,7 +2,7 @@ module Core.Slice.Iter
 
 open Rust_primitives
 
-let t_Chunks a = slice (slice a)
-let t_ChunksExact a = slice (slice a)
-let t_Iter a = slice a
+let t_Chunks a = t_Slice (t_Slice a)
+let t_ChunksExact a = t_Slice (t_Slice a)
+let t_Iter a = t_Slice a
 
