libs/fstar/core/Core.Array.fst
@@ -1,5 +1,7 @@
 module Core.Array
 open Rust_primitives
 
-let impl_23__map #n (arr: array 'a n) (f: 'a -> 'b): array 'b n 
+type t_TryFromSliceError = | TryFromSliceError
+
+let impl_23__map #n (arr: t_Array 'a n) (f: 'a -> 'b): t_Array 'b n 
   = map_array arr f
