libs/fstar/core/Core.Num.fsti
@@ -3,30 +3,30 @@ open Rust_primitives
 
 let impl__u32__wrapping_add: u32 -> u32 -> u32 = add_mod
 val impl__u32__rotate_left: u32 -> u32 -> u32
-val impl__u32__from_le_bytes: array u8 (sz 4) -> u32
-val impl__u32__from_be_bytes: array u8 (sz 4) -> u32
-val impl__u32__to_le_bytes: u32 -> array u8 (sz 4)
-val impl__u32__to_be_bytes: u32 -> array u8 (sz 4)
+val impl__u32__from_le_bytes: t_Array u8 (sz 4) -> u32
+val impl__u32__from_be_bytes: t_Array u8 (sz 4) -> u32
+val impl__u32__to_le_bytes: u32 -> t_Array u8 (sz 4)
+val impl__u32__to_be_bytes: u32 -> t_Array u8 (sz 4)
 val impl__u32__rotate_right: u32 -> u32 -> u32
 
 
 open FStar.UInt64
 let impl__u64__wrapping_add: u64 -> u64 -> u64 = add_underspec
 val impl__u64__rotate_left: u32 -> u32 -> u32
-val impl__u64__from_le_bytes: array u8 (sz 8) -> u64
-val impl__u64__from_be_bytes: array u8 (sz 8) -> u64
-val impl__u64__to_le_bytes: u64 -> array u8 (sz 8)
-val impl__u64__to_be_bytes: u64 -> array u8 (sz 8)
+val impl__u64__from_le_bytes: t_Array u8 (sz 8) -> u64
+val impl__u64__from_be_bytes: t_Array u8 (sz 8) -> u64
+val impl__u64__to_le_bytes: u64 -> t_Array u8 (sz 8)
+val impl__u64__to_be_bytes: u64 -> t_Array u8 (sz 8)
 val impl__u64__rotate_right: u64 -> u64 -> u64
 
 
 open FStar.UInt128
 let impl__u128__wrapping_add (x: u128) (y: u128): u128 = add_underspec x y
 val impl__u128__rotate_left: u128 -> u128 -> u128
-val impl__u128__from_le_bytes: array u8 (sz 16) -> u128
-val impl__u128__from_be_bytes: array u8 (sz 16) -> u128
-val impl__u128__to_le_bytes: u128 -> array u8 (sz 16)
-val impl__u128__to_be_bytes: u128 -> array u8 (sz 16)
+val impl__u128__from_le_bytes: t_Array u8 (sz 16) -> u128
+val impl__u128__from_be_bytes: t_Array u8 (sz 16) -> u128
+val impl__u128__to_le_bytes: u128 -> t_Array u8 (sz 16)
+val impl__u128__to_be_bytes: u128 -> t_Array u8 (sz 16)
 val impl__u128__rotate_right: u128 -> u128 -> u128
 
 val impl__u8__pow: u8 -> u32 -> u8
