libs/fstar/core/Core.Ops.Deref.fst
@@ -1,3 +1,3 @@
 module Core.Ops.Deref
 
-let deref = id
+let f_deref = id
