libs/fstar/core/Core.Ops.Index.fst
@@ -6,3 +6,11 @@ class t_Index t_Self t_Idx = {
   f_index: s:t_Self -> i:t_Idx{in_range s i} -> f_Output;
 }
 
+open Rust_primitives
+open Core.Ops.Index
+
+instance impl__index t l n: t_Index (t_Array t l) (int_t n)
+  = { f_Output = t;
+      in_range = (fun (s: t_Array t l) (i: int_t n) -> v i >= 0 && v i < v l);
+      f_index = (fun s i -> Seq.index s (v i));
+    }
