libs/fstar/core/Core.Slice.fsti
@@ -1,23 +1,24 @@
 module Core.Slice
-open Rust_primitives
+open Rust_primitives.Arrays
+open Rust_primitives.Integers
 
-let impl__len (s: slice 'a)
+let impl__len (s: t_Slice 'a)
   : len: usize {len == sz (Seq.length s)} = 
   sz (Seq.length s)
 
 open Core.Slice.Iter
 
-val impl__chunks (x: slice 'a) (cs: usize): t_Chunks 'a
+val impl__chunks (x: t_Slice 'a) (cs: usize): t_Chunks 'a
 
-let impl__iter (s: slice 't): slice 't = s
+let impl__iter (s: t_Slice 't): t_Slice 't = s
 
-val impl__chunks_exact (x: slice 'a) (cs: usize): t_ChunksExact 'a
+val impl__chunks_exact (x: t_Slice 'a) (cs: usize): t_ChunksExact 'a
 
 open Core.Ops.Index
 
-instance impl__index t: t_Index (slice t) usize
+instance impl__index t n: t_Index (t_Slice t) (int_t n)
   = { f_Output = t;
-      in_range = (fun (s: slice t) (i: usize) -> i <. length s);
+      in_range = (fun (s: t_Slice t) (i: int_t n) -> v i >= 0 && v i < v (length s));
       f_index = (fun s i -> Seq.index s (v i));
     }
 
