libs/fstar/rust_primitives/Rust_primitives.fst
@@ -3,6 +3,15 @@ module Rust_primitives
 include Rust_primitives.Integers
 include Rust_primitives.Arrays
 
+class cast_tc a b = {
+  cast: a -> b; 
+}
+
+/// Rust's casts operations on integers are non-panicking
+instance cast_tc_integers (t:inttype) (t':inttype)
+  : cast_tc (int_t t) (int_t t')
+  = { cast = (fun x -> Rust_primitives.Integers.cast_mod #t #t' x) }
+
 class unsize_tc source = {
   output: Type;
   unsize: source -> output;
